UniverseAbstractions/Axioms/Universe/Properties.lean
@@ -1,0 +1,88 @@
+import UniverseAbstractions.Axioms.Universes
+import UniverseAbstractions.Axioms.Universe.Functors
+
+import mathlib4_experiments.Data.Equiv.Basic
+
+
+
+set_option autoBoundImplicitLocal false
+--set_option pp.universes true
+
+universe u v w
+
+
+
+-- We define a "`V`-valued property" on a type `α` to be a functor targetting a universe `V`. If
+-- `V` is the universe `prop`, this is just a regular property, or equivalently `Set α` in Lean.
+
+class HasGeneralizedProperties (U : Universe.{u})
+  extends HasFunctoriality.{u, v + 1, w} U univ.{v}, HasConstFun U univ.{v}
+
+namespace HasGeneralizedProperties
+
+  variable {U : Universe.{u}} [HasGeneralizedProperties.{u, v, w} U]
+
+  def Property (V : univ.{v}) (α : U) : Sort (max u (v + 1) w) := α ⟶' V
+
+  variable {V : univ.{v}}
+
+  instance coeFun {α : U} : CoeFun (Property V α) (λ _ => α → V) := HasFunctoriality.coeFun
+
+  section Properties
+
+    variable {α : U} (P : Property V α)
+
+    -- Universality and existence with respect to generalized properties are given by `∀` and `Σ'`.
+
+    def Pi    : Sort (imax u v)  := ∀  a, ⌈P a⌉
+    def Sigma : Sort (max 1 u v) := Σ' a, ⌈P a⌉
+
+    class IsUniversal where
+    (h : Pi P)
+
+    class IsInhabited where
+    (h : Sigma P)
+
+  end Properties
+
+  -- Given a type `β : V`, we can define a constant property that always yields this type. `Pi`
+  -- applied to this property is just the type of functions from `α` to `β`, and `Sigma` applied to
+  -- this property is just the product of `α` and `β`.
+
+  def constProp (α : U) (β : V) : Property V α := HasConstFun.constFun' α β
+
+  namespace constProp
+
+    variable (α : U) (β : V)
+
+    def piEquivFun : Pi (constProp α β) ≃ (α → β) := Equiv.refl (α → β)
+
+    def sigmaEquivProd : Sigma (constProp α β) ≃ PProd ⌈α⌉ ⌈β⌉ :=
+    { toFun    := λ s => ⟨s.fst, s.snd⟩,
+      invFun   := λ p => ⟨p.fst, p.snd⟩,
+      leftInv  := λ ⟨_, _⟩ => rfl,
+      rightInv := λ ⟨_, _⟩ => rfl }
+
+  end constProp
+
+end HasGeneralizedProperties
+
+
+
+-- We can define a "`V`-valued set" with base universe `U` as a bundled version of `Property V`
+-- when treated as a type class on `U`. In other words, a set is a type `α : U` together with a
+-- `V`-valued property `P` on `α`.
+--
+-- This gives us a universe of all `V`-valued sets with base universe `U`, where we can define
+-- functors etc.
+--
+-- (TODO: How does this relate to embedded sigma types, i.e. subtypes?)
+
+def HasGeneralizedProperties.asTypeClass (U : Universe.{u}) [HasGeneralizedProperties.{u, v, w} U]
+                                         (V : Universe.{v}) :
+  GeneralizedTypeClass ⌈U⌉ :=
+HasGeneralizedProperties.Property V
+
+def GeneralizedSet (U : Universe.{u}) [HasGeneralizedProperties.{u, v, w} U] (V : Universe.{v}) :
+  Type (max u (v + 1) w) :=
+Bundled (HasGeneralizedProperties.asTypeClass U V)
