UniverseAbstractions/Axioms/Universe/Quantifiers.lean
@@ -1,0 +1,73 @@
+import UniverseAbstractions.Axioms.Universes
+import UniverseAbstractions.Axioms.Universe.Functors
+import UniverseAbstractions.Axioms.Universe.Properties
+
+
+
+set_option autoBoundImplicitLocal false
+--set_option pp.universes true
+
+universe u v w w'
+
+
+
+-- TODO require const pi to functor
+
+class HasUniversality (U : Universe.{u}) [HasGeneralizedProperties.{u, v, w} U] (V : Universe.{v}) :
+  Type (max u v w) where
+(IsUniv {α : U} {P : HasGeneralizedProperties.Property V α} : HasGeneralizedProperties.Pi P → Sort w)
+
+namespace HasUniversality
+
+  structure Pi {U : Universe.{u}} [HasGeneralizedProperties.{u, v, w} U] {V : Universe.{v}}
+               [h : HasUniversality.{u, v, w} U V] {α : U} (P : HasGeneralizedProperties.Property V α) :
+    Sort (max 1 u v w) where
+  (f      : HasGeneralizedProperties.Pi P)
+  (isUniv : h.IsUniv f)
+
+  variable {U : Universe.{u}} [HasGeneralizedProperties.{u, v, w} U] {V : Universe.{v}}
+           [h : HasUniversality.{u, v, w} U V] {α : U} (P : HasGeneralizedProperties.Property V α)
+
+  instance coeFun : CoeFun (Pi P) (λ _ => HasGeneralizedProperties.Pi P) := ⟨Pi.f⟩
+
+end HasUniversality
+
+
+
+class HasPiTypes (U : Universe.{u}) [HasGeneralizedProperties.{u, v, w'} U] (V : Universe.{v})
+                 (W : outParam Universe.{w})
+  extends HasUniversality.{u, v, w'} U V : Type (max u v w w') where
+[embed {α : U} (P : HasGeneralizedProperties.Property V α) : HasEmbeddedType.{w, max 1 u v w'} W (HasUniversality.Pi P)]
+
+namespace HasPiTypes
+
+  variable {U : Universe} [HasGeneralizedProperties U] {V W : Universe} [h : HasPiTypes U V W]
+
+  instance hasEmbeddedType {α : U} (P : HasGeneralizedProperties.Property V α) :
+    HasEmbeddedType W (HasUniversality.Pi P) :=
+  h.embed P
+
+  def Pi {α : U} (P : HasGeneralizedProperties.Property V α) : W :=
+  HasEmbeddedType.EmbeddedType W (HasUniversality.Pi P)
+
+  variable {α : U} {P : HasGeneralizedProperties.Property V α}
+
+  def toExternal   (F : Pi P)                 : HasUniversality.Pi P := HasEmbeddedType.toExternal   W F
+  def fromExternal (F : HasUniversality.Pi P) : Pi P                 := HasEmbeddedType.fromExternal W F
+
+  def funCoe (F : Pi P) : HasGeneralizedProperties.Pi P := (toExternal F).f
+  instance coeFun : CoeFun ⌈Pi P⌉ (λ _ => HasGeneralizedProperties.Pi P) := ⟨funCoe⟩
+
+  @[simp] theorem fromToExternal (F : Pi P)                 : fromExternal (toExternal F) = F := HasEmbeddedType.fromToExternal W F
+  @[simp] theorem toFromExternal (F : HasUniversality.Pi P) : toExternal (fromExternal F) = F := HasEmbeddedType.toFromExternal W F
+
+  @[simp] theorem toExternal.eff   (F : Pi P)                 (a : α) : (toExternal   F) a = F a := rfl
+  @[simp] theorem fromExternal.eff (F : HasUniversality.Pi P) (a : α) : (fromExternal F) a = F a :=
+  congrFun (congrArg HasUniversality.Pi.f (toFromExternal F)) a
+
+end HasPiTypes
+
+
+
+class HasEmbeddedPiTypes (U : Universe.{u}) [HasGeneralizedProperties.{u, v, w} U] (V : Universe.{v})
+  extends HasPiTypes.{u, v, v, w} U V V
